Introduce sinv

nola/iris/inv.v
@@ -1,52 +1,39 @@
 (** * Nola later-free invariant *)
 
-From nola.iris Require Export upd.
+From nola.iris Require Export sinv upd.
 From stdpp Require Export namespaces.
 From iris.algebra Require Import gset.
-From iris.base_logic.lib Require Import ghost_map wsat invariants.
+From iris.base_logic.lib Require Import wsat invariants.
 From iris.proofmode Require Import proofmode.
 
 Implicit Type PROP : Type.
 
 (** ** Resources *)
 
-Class ninvGS PROP Σ := NinvGS {
-  ninvGS_in :: ghost_mapG Σ positive (leibnizO PROP);
-  ninv_name : gname;
-}.
-Class ninvGpreS PROP Σ :=
-  ninvGpreS_in :: ghost_mapG Σ positive (leibnizO PROP).
-Definition ninvΣ PROP : gFunctors := ghost_mapΣ positive (leibnizO PROP).
+Class ninvGS PROP Σ := ninvGS_in :: sinvGS PROP Σ.
+Class ninvGpreS PROP Σ := ninvGpreS_in :: sinvGpreS PROP Σ.
+Definition ninvΣ PROP : gFunctors := sinvΣ PROP.
 #[export] Instance subG_ninvΣ `{!subG (ninvΣ PROP) Σ} : ninvGpreS PROP Σ.
 Proof. solve_inG. Qed.
 
 Section ninv.
   Context `{!invGS_gen hlc Σ, !ninvGS PROP Σ}.
 
-  (** ** Propositions *)
-
-  (** [ownI]: Basic invariant token *)
-  Local Definition ownI (i : positive) (P : PROP) : iProp Σ :=
-    i ↪[ninv_name]□ P.
-
   (** [ninv]: Invariant token *)
   Local Definition ninv_def (N : namespace) (P : PROP) : iProp Σ :=
-    ∃ i, ⌜i ∈ (↑N:coPset)⌝ ∗ ownI i P.
+    ∃ i, ⌜i ∈ (↑N:coPset)⌝ ∗ sinv_tok' i P.
   Local Definition ninv_aux : seal ninv_def. Proof. by eexists. Qed.
   Definition ninv := ninv_aux.(unseal).
   Local Lemma ninv_unseal : ninv = ninv_def. Proof. exact: seal_eq. Qed.
 
-  (** [ninv] is timeless and persistent *)
-  #[export] Instance ninv_timeless {N P} : Timeless (ninv N P).
-  Proof. rewrite ninv_unseal. exact _. Qed.
+  (** [ninv] is persistent and timeless *)
   #[export] Instance ninv_persistent {N P} : Persistent (ninv N P).
   Proof. rewrite ninv_unseal. exact _. Qed.
+  #[export] Instance ninv_timeless {N P} : Timeless (ninv N P).
+  Proof. rewrite ninv_unseal. exact _. Qed.
 
-  (** [ninv_wsat]: Invariant world satisfaction *)
-  Local Definition authI (I : gmap positive PROP) :=
-    ghost_map_auth ninv_name 1 I.
   Local Definition ninv_wsat_def (intp : PROP -d> iProp Σ) : iProp Σ :=
-    ∃ I, authI I ∗ [∗ map] i ↦ P ∈ I, intp P ∗ ownD {[i]} ∨ ownE {[i]}.
+    sinv_wsat' (λ i P, intp P ∗ ownD {[i]} ∨ ownE {[i]})%I.
   Local Definition ninv_wsat_aux : seal ninv_wsat_def. Proof. by eexists. Qed.
   Definition ninv_wsat := ninv_wsat_aux.(unseal).
   Local Lemma ninv_wsat_unseal : ninv_wsat = ninv_wsat_def.
@@ -60,64 +47,28 @@ Section ninv.
 
   (** ** Lemmas *)
 
-  (** Allocate [ownI] *)
-  Local Lemma ownI_alloc_rec {intp P N} :
-    (∀ i, ⌜i ∈ (↑N:coPset)⌝ → ownI i P -∗ intp P) -∗ ninv_wsat intp ==∗
-      ∃ i, ⌜i ∈ (↑N:coPset)⌝ ∗ ninv_wsat intp ∗ ownI i P.
-  Proof.
-    rewrite ninv_wsat_unseal. iIntros "→P [%I[I W]]".
-    iMod (own_unit (gset_disjUR positive) disabled_name) as "D".
-    iMod (own_updateP with "[$]") as (x) "[X D]".
-    { apply (gset_disj_alloc_empty_updateP_strong'
-        (λ i, I !! i = None ∧ i ∈ (↑N:coPset)))=> E.
-      case: (fresh_inv_name (E ∪ dom I) N)=>
-        [i[/not_elem_of_union[?/not_elem_of_dom ?]?]]. by exists i. }
-    iDestruct "X" as %[i[->[??]]].
-    iMod (ghost_map_insert_persist with "I") as "[I #i]"; [done|]. iModIntro.
-    iExists _. iFrame "i". iSplit; [done|]. iExists _. iFrame "I".
-    iApply (big_sepM_insert_2 with "[→P D]"); [|done]. iLeft.
-    iSplitR "D"; [|done]. by iApply "→P".
-  Qed.
-  (** Turn [ownI] to [ninv] *)
-  Local Lemma ownI_ninv {i N P} : i ∈ (↑N:coPset) → ownI i P ⊢ ninv N P.
-  Proof. rewrite ninv_unseal. iIntros. iExists _. by iSplit. Qed.
   (** Allocate [ninv] *)
   Lemma ninv_alloc_rec {intp N P} :
     (ninv N P -∗ intp P) =[ninv_wsat intp]=∗ ninv N P.
   Proof.
-    iIntros "→P W".
-    iMod (ownI_alloc_rec with "[→P] W") as (i ?) "[W i]".
-    - iIntros (i ?) "i". iApply "→P". by iApply ownI_ninv.
-    - iModIntro. iFrame "W". by iApply ownI_ninv.
+    rewrite ninv_unseal ninv_wsat_unseal. iIntros "→P W".
+    iDestruct (sinv_alloc' with "W") as (I) "big".
+    iMod (own_unit (gset_disjUR positive) disabled_name) as "D".
+    iMod (own_updateP with "[$]") as (x) "[X D]".
+    { apply (gset_disj_alloc_empty_updateP_strong'
+        (λ i, i ∉ I ∧ i ∈ (↑N:coPset)))=> J.
+      case: (fresh_inv_name (I ∪ J) N)=> [i[/not_elem_of_union[??]?]].
+      by exists i. }
+    iDestruct "X" as %[i[->[??]]]. iMod ("big" with "[//]") as "[#i →W]".
+    iModIntro. iSplitL; [|iExists _; by iSplit]. iApply "→W". iLeft.
+    iSplitR "D"; [|done]. iApply "→P". iExists _; by iSplit.
   Qed.
   Lemma ninv_alloc {intp N P} : intp P =[ninv_wsat intp]=∗ ninv N P.
   Proof. iIntros "P W". iApply (ninv_alloc_rec with "[P] W"). by iIntros. Qed.
 
-  (** Open by [ownI] *)
-  Local Lemma ownI_open {intp i P} :
-    ownI i P -∗ ownE {[i]} -∗ ninv_wsat intp -∗
-      ninv_wsat intp ∗ intp P ∗ ownD {[i]}.
-  Proof.
-    rewrite ninv_wsat_unseal. iIntros "i ? [%I[I W]]".
-    iDestruct (ghost_map_lookup with "I i") as %?.
-    iDestruct (big_sepM_lookup_acc with "W") as "[[[$$]|?] →W]";
-      [done| |iDestruct (ownE_singleton_twice with "[$]") as "[]"].
-    iExists _. iFrame "I". iApply "→W". by iRight.
-  Qed.
-  (** Close by [ownI] *)
-  Local Lemma ownI_close {intp i P} :
-    ownI i P -∗ ownD {[i]} -∗ intp P -∗ ninv_wsat intp -∗
-      ninv_wsat intp ∗ ownE {[i]}.
-  Proof.
-    rewrite ninv_wsat_unseal. iIntros "i ? ? [%I[I W]]".
-    iDestruct (ghost_map_lookup with "I i") as %?.
-    iDestruct (big_sepM_lookup_acc with "W") as "[[[_ ?]|$] →W]";
-      [done|iDestruct (ownD_singleton_twice with "[$]") as %[]|].
-    iExists _. iFrame "I". iApply "→W". iLeft. iFrame.
-  Qed.
   (** Access [ownE] *)
   Local Lemma ownE_acc {N E} :
-    ↑N ⊆ E →  ⊢ |={E,E∖↑N}=> ownE (↑N) ∗ (ownE (↑N) ={E∖↑N,E}=∗ True).
+    ↑N ⊆ E → ⊢ |={E,E∖↑N}=> ownE (↑N) ∗ (ownE (↑N) ={E∖↑N,E}=∗ True).
   Proof.
     rewrite fancy_updates.uPred_fupd_unseal /fancy_updates.uPred_fupd_def.
     move=> ?. iIntros "[$ E]". do 2 iModIntro.
@@ -129,20 +80,25 @@ Section ninv.
     ↑N ⊆ E → ninv N P =[ninv_wsat intp]{E,E∖↑N}=∗
       intp P ∗ (intp P =[ninv_wsat intp]{E∖↑N,E}=∗ True)%I.
   Proof.
-    move=> ?. rewrite ninv_unseal. iIntros "[%i[% #i]] W".
+    move=> ?. rewrite ninv_unseal ninv_wsat_unseal. iIntros "[%i[% #i]] W".
     iMod ownE_acc as "[N cl]"; [done|].
+    iDestruct (sinv_acc' with "i W") as "[in →W]".
     rewrite {1 2}(union_difference_L {[i]} (↑N)); [|set_solver].
-    rewrite ownE_op; [|set_solver]. iDestruct "N" as "[E E']".
-    iDestruct (ownI_open with "i E W") as "[$[$ D]]". iModIntro.
-    iIntros "P W". iDestruct (ownI_close with "i D P W") as "[$ E]".
-    iApply "cl". iFrame.
+    rewrite ownE_op; [|set_solver]. iDestruct "N" as "[Ei EN∖i]".
+    iDestruct "in" as "[[$ D]|Ei']"; last first.
+    { iDestruct (ownE_singleton_twice with "[$Ei $Ei']") as "[]". }
+    iModIntro. iDestruct ("→W" with "[$Ei]") as "$". iIntros "P W".
+    iDestruct (sinv_acc' with "i W") as "[[[_ D']|Ei] →W]".
+    { iDestruct (ownD_singleton_twice with "[$D $D']") as "[]". }
+    iMod ("cl" with "[$Ei $EN∖i]") as "_". iModIntro. iSplitL; [|done].
+    iApply "→W". iLeft. iFrame.
   Qed.
 End ninv.
 
 (** Allocate [ninv_wsat] *)
-Lemma ninv_wsat_alloc `{!invGS_gen hlc Σ, !ninvGpreS PROP Σ} :
+Lemma ninv_wsat_alloc `{!ninvGpreS PROP Σ, !invGS_gen hlc Σ} :
   ⊢ |==> ∃ _ : ninvGS PROP Σ, ∀ intp, ninv_wsat intp.
 Proof.
-  iMod ghost_map_alloc_empty as (γ) "●". iModIntro. iExists (NinvGS _ _ _ γ).
-  rewrite ninv_wsat_unseal. iIntros (?). iExists ∅. by iFrame.
+  iMod sinv_wsat_alloc as (?) "W". iModIntro. iExists _. iIntros (?).
+  rewrite ninv_wsat_unseal. iApply "W".
 Qed.
