nola/iris/sinv.v
@@ -1,0 +1,114 @@
+(** * Simple invariant *)
+
+From nola.iris Require Export upd.
+From iris.base_logic.lib Require Import ghost_map.
+From iris.proofmode Require Import proofmode.
+
+Implicit Type PROP : Type.
+
+Class sinvGS PROP Σ := SinvGS {
+  sinvGS_in :: ghost_mapG Σ positive (leibnizO PROP);
+  sinv_name : gname;
+}.
+Class sinvGpreS PROP Σ :=
+  sinvGpreS_in :: ghost_mapG Σ positive (leibnizO PROP).
+Definition sinvΣ PROP : gFunctors := ghost_mapΣ positive (leibnizO PROP).
+#[export] Instance subG_sinvΣ `{!subG (sinvΣ PROP) Σ} : sinvGpreS PROP Σ.
+Proof. solve_inG. Qed.
+
+Section sinv.
+  Context `{!sinvGS PROP Σ}.
+
+  (** Simple invariant token *)
+  Local Definition sinv_tok'_def i P : iProp Σ := i ↪[sinv_name]□ P.
+  Local Lemma sinv_tok'_aux : seal sinv_tok'_def. Proof. by eexists. Qed.
+  Definition sinv_tok' := sinv_tok'_aux.(unseal).
+  Local Lemma sinv_tok'_unseal : sinv_tok' = sinv_tok'_def.
+  Proof. exact: seal_eq. Qed.
+  Local Definition sinv_tok_def P : iProp Σ := ∃ i, sinv_tok' i P.
+  Local Lemma sinv_tok_aux : seal sinv_tok_def. Proof. by eexists. Qed.
+  Definition sinv_tok := sinv_tok_aux.(unseal).
+  Local Lemma sinv_tok_unseal : sinv_tok = sinv_tok_def.
+  Proof. exact: seal_eq. Qed.
+
+  (** World satisfaction *)
+  Definition sinv_wsat'_def intp : iProp Σ :=
+    ∃ M, ghost_map_auth sinv_name 1 M ∗ [∗ map] i ↦ P ∈ M, intp i P.
+  Local Lemma sinv_wsat'_aux : seal sinv_wsat'_def. Proof. by eexists. Qed.
+  Definition sinv_wsat' := sinv_wsat'_aux.(unseal).
+  Local Lemma sinv_wsat'_unseal : sinv_wsat' = sinv_wsat'_def.
+  Proof. exact: seal_eq. Qed.
+End sinv.
+Notation sinv_wsat intp := (sinv_wsat' (λ _, intp)).
+
+Section sinv.
+  Context `{!sinvGS PROP Σ}.
+  Implicit Type (i : positive) (P : PROP) (I : gset positive).
+
+  (** [sinv_tok'] and [sinv_tok] are persistent and timeless *)
+  #[export] Instance sinv_tok'_persistent {i P} : Persistent (sinv_tok' i P).
+  Proof. rewrite sinv_tok'_unseal. exact _. Qed.
+  #[export] Instance sinv_tok'_timeless {i P} : Timeless (sinv_tok' i P).
+  Proof. rewrite sinv_tok'_unseal. exact _. Qed.
+  #[export] Instance sinv_tok_persistent {P} : Persistent (sinv_tok P).
+  Proof. rewrite sinv_tok_unseal. exact _. Qed.
+  #[export] Instance sinv_tok_timeless {P} : Timeless (sinv_tok P).
+  Proof. rewrite sinv_tok_unseal. exact _. Qed.
+
+  (** [sinv_wsat'] is non-expansive *)
+  #[export] Instance sinv_wsat'_ne {n} :
+    Proper (pointwise_relation _ (pointwise_relation _ (≡{n}≡)) ==> (≡{n}≡))
+      sinv_wsat'.
+  Proof. rewrite sinv_wsat'_unseal. solve_proper. Qed.
+  #[export] Instance sinv_wsat'_proper :
+    Proper (pointwise_relation _ (pointwise_relation _ (≡)) ==> (≡)) sinv_wsat'.
+  Proof. rewrite sinv_wsat'_unseal. solve_proper. Qed.
+
+  (** [sinv_wsat'] is timeless if [intp] is always timeless *)
+  #[export] Instance sinv_wsat'_timeless `{!∀ i P, Timeless (intp i P)} :
+    Timeless (sinv_wsat' intp).
+  Proof. rewrite sinv_wsat'_unseal. exact _. Qed.
+
+  (** Allocate [sinv_tok'] *)
+  Lemma sinv_alloc' {intp} P :
+    sinv_wsat' intp -∗ ∃ I, ∀ i, ⌜i ∉ I⌝ ==∗
+      sinv_tok' i P ∗ (intp i P -∗ sinv_wsat' intp).
+  Proof.
+    rewrite sinv_wsat'_unseal. iIntros "[%M[● M]]". iExists (dom M).
+    iIntros (i ?). iMod (ghost_map_insert_persist with "●") as "[● #i]";
+      [by apply not_elem_of_dom|]. iModIntro.
+    iSplitR; [by rewrite sinv_tok'_unseal|]. iIntros "P". iExists _. iFrame "●".
+    iApply (big_sepM_insert_2 with "P M").
+  Qed.
+  Lemma sinv_alloc {intp} P :
+    sinv_wsat intp ==∗ sinv_tok P ∗ (intp P -∗ sinv_wsat intp).
+  Proof.
+    iIntros "W". iDestruct (sinv_alloc' with "W") as (?) "big".
+    iMod ("big" with "[]") as "[? $]". { iPureIntro. apply is_fresh. }
+    iModIntro. rewrite sinv_tok_unseal. by iExists _.
+  Qed.
+
+  (** Accesss via [sinv_tok] *)
+  Lemma sinv_acc' {intp i P} :
+    sinv_tok' i P -∗ sinv_wsat' intp -∗
+      intp i P ∗ (intp i P -∗ sinv_wsat' intp).
+  Proof.
+    rewrite sinv_tok'_unseal sinv_wsat'_unseal. iIntros "i [%M[● M]]".
+    iDestruct (ghost_map_lookup with "● i") as %?.
+    iDestruct (big_sepM_lookup_acc with "M") as "[$ →M]"; [done|]. iIntros "P".
+    iExists _. iFrame "●". by iApply "→M".
+  Qed.
+  Lemma sinv_acc {intp P} :
+    sinv_tok P -∗ sinv_wsat intp -∗ intp P ∗ (intp P -∗ sinv_wsat intp).
+  Proof.
+    rewrite sinv_tok_unseal. iIntros "[%i i]". iApply (sinv_acc' with "i").
+  Qed.
+End sinv.
+
+(** Allocate [sinv_wsat] *)
+Lemma sinv_wsat_alloc `{!sinvGpreS PROP Σ} :
+  ⊢ |==> ∃ _ : sinvGS PROP Σ, ∀ intp, sinv_wsat' intp.
+Proof.
+  iMod ghost_map_alloc_empty as (γ) "●". iModIntro. iExists (SinvGS _ _ _ γ).
+  iIntros. rewrite sinv_wsat'_unseal. iExists ∅. by iFrame.
+Qed.
