README.md
@@ -67,7 +67,8 @@ All the Coq code is in [`nola/`](nola/) and structured as follows:
   + [`deriv`](nola/iris/deriv.v) (Derivability)
   + [`upd`](nola/iris/upd.v) (Update),
     [`wp`](nola/iris/wp.v) (Weakest precondition)
-  + [`inv`](nola/iris/inv.v) (Invariant),
+  + [`sinv`](nola/iris/sinv.v) (Simple invariant),
+    [`inv`](nola/iris/inv.v) (Invariant),
     [`na_inv`](nola/iris/na_inv.v) (Non-atomic invariant)
   + [`lft`](nola/iris/lft.v) (Lifetime),
     [`borrow`](nola/iris/borrow.v) (Borrowing)
